theories/nonintereference.v
@@ -1,0 +1,1593 @@
+
+Set Implicit Arguments.
+Unset Strict Implicit.
+Unset Printing Implicit Defensive.
+
+Require Import RelationClasses.
+From Paco Require Import paco.
+From mathcomp Require Import all_ssreflect.
+From mathcomp Require Import order.
+Require Import Streams.
+From HB Require Import structures.
+From deriving Require Import deriving.
+Require Import Coq.Program.Equality.
+From Equations Require Import Equations.
+Require Import Coq.Classes.DecidableClass.
+Import Order.TTheory.
+Open Scope order_scope.
+
+Require Export NonInterference.theories.models.
+
+(*We start by showing that model1 is interfering*)
+Definition ir_dis (l : level) (ir : [TInterrupt]) := ir = DiskInterrupt /\ l = \bot.
+Definition TInterrupt_rel : myrel [TInterrupt].
+  refine (@MyRel _
+            ir_dis
+            (fun l ir ir' => ir = ir' \/ ir_dis l ir /\ ir_dis l ir')
+            _
+            _
+            _
+            _).
+  ssa. con. intro. ssa. intro. ssa. de H.
+  intro. ssa. de H. de H0. subst. ssa. subst.
+  eauto. de H0. subst. ssa.
+  ssa. de H0. eauto. move: H0 H1. rewrite /ir_dis. ssa.
+  subst. eauto.
+  ssa. move: H0. rewrite /ir_dis. ssa. subst.
+  rewrite /order in H. rewrite lex0 in H. apply/eqP. done.
+  ssa. rewrite /ir_dis. con. ssa. ssa. de H0. subst.
+  move:H. rewrite /ir_dis. intros;subst. ssa.
+  ssa. de H0. move: H. rewrite /ir_dis. ssa.
+Defined.  
+
+
+Definition in_rel : myrel [T_in] := TInterrupt_rel.
+
+Definition out_rel : myrel [T_out'] := eqpair (eqmaybe (publicRel _))
+                                          (eqpair (eqmaybe (semiprivateRel _))
+                                             (eqpair (eqmaybe (publicRel _))
+                                                (eqpair (eqmaybe_top ((semiprivateRel _)))
+                                                   (eqpair (eqmaybe_top (semiprivateRel _))
+                                                      (eqmaybe (publicRel _)))))).
+
+Lemma Trace_imp : forall (A B : Ty) (p : Proc A B) (s : seq ([A] + [B])) l (BRel BRel' : myrel [B]), (forall x y, rel BRel l x y -> rel BRel' l x y) -> Trace BRel l s p -> Trace BRel' l s p.
+Proof.  
+  intros.
+  elim : H0 H;ssa.
+  econ. eauto. eauto.
+  econ;eauto.
+Qed.
+
+Lemma helper_trace' : Trace (publicRel _) \bot [::pub_get';pub_get'] model_bad.
+Proof.
+    rewr;simpl;rewr;simpl;rewr;simpl;rewr.
+    (first [econ;[idtac | econ | idtac] | econ];
+     reduce_tac;try solve [reflexivity| reduce_tac;reduce_tac];simpl;try swi_instans).
+    simpl.
+
+   (first [econ;[idtac | econ | idtac] | econ];
+    reduce_tac2;try solve [reflexivity| reduce_tac2;reduce_tac2];simpl;try swi_instans).
+   econ. reduce_tac2;reduce_tac2. econ. econ. reduce_tac. econ. econ.
+   reduce_tac. econ. econ. reduce_tac. econ. econ. reduce_tac. econ.
+   econ. reduce_tac. econ. econ. reduce_tac. econ.
+Qed.   
+
+Lemma helper_trace : Trace out_rel \bot [::pub_get';pub_get'] model_bad.
+Proof.
+  eapply Trace_imp. 2:eapply helper_trace'.
+  intros. simpl in H. subst. auto.
+Qed.  
+
+
+(*Opaque otherwise the inversion tactic take forever*)
+Opaque state_step f_si initial_state def f_proj.
+
+Lemma model_bad_not_NI : ~ NI in_rel out_rel model_bad.
+Proof.
+  intro. rewrite /NI in H. move: (H \bot). clear H.
+  rewrite /NI_l. case=>_ [] + _. intros.
+  move: helper_trace.
+  move/a. move/(_ (DiskInterrupt) 0). simpl.
+  have: ir_dis \bot DiskInterrupt. ssa.
+  move=>aa. move/(_ aa).
+  move=>Htr. clear a aa.
+  inv Htr;clear Htr;match_dd. 
+  rewrite /= in x. clear x.
+  inv H3;clear H3;match_dd. ssa.
+  inv H5;clear H5;match_dd.
+  move: H9. clear. simpl. ssa.
+Qed.
+
+Transparent f_si initial_state def f_proj.
+
+
+(*The rest of the file shows nonintereference of model2 and model3*)
+
+Lemma eqsum_L_llrr l i i' : rel (eqsum_L in_rel out_rel) l i i' -> is_inl i /\ is_inl i' \/ is_inr i /\ is_inr i'.
+Proof.
+  intros. destruct i. destruct i'. ssa.
+  exfalso. ssa. destruct i'. ssa. ssa.
+Qed.
+
+Lemma eqsum_llrr  (A B : Ty) (ARel : myrel [A]) (BRel : myrel [B])  l i i' : rel (eqsum ARel BRel) l i i' -> is_inl i /\ is_inl i' \/ is_inr i /\ is_inr i'.
+Proof.
+  intros. destruct i. destruct i'. ssa.
+  exfalso. ssa. destruct i'. ssa. ssa.
+Qed.
+
+Lemma eqsum_split (A B : Ty) (ARel : myrel [A]) (BRel : myrel [B]) l i0 i1 : rel (eqsum ARel BRel) l i0 i1 -> (exists i0' i1', (i0 = inl i0' /\ i1 = inl i1' /\ rel ARel l i0' i1')) \/
+                                                                                                              exists i0' i1', (i0 = inr i0' /\ i1 = inr i1' /\ rel BRel l i0' i1').
+Proof.
+  intros. apply eqsum_llrr in H as H'. destruct H'.
+  destruct H0. destruct i0. destruct i1.
+  left. exists i. exists i0. ssa.
+  ssa. ssa. destruct i0. ssa.
+  destruct i1. ssa.
+  right. exists i. exists i0. ssa.
+Qed.
+
+Lemma semiprivate_not_bot : forall (A : Ty) l (x y : [A]), l <> \bot -> x = y -> rel (semiprivateRel _) l x y.
+Proof.
+ssa.
+Qed.
+
+Lemma semiprivate_not_bot' : forall (A : Ty) l (x y : [A]), l <> \bot -> rel (semiprivateRel _) l x y -> x = y.
+Proof.
+ssa. de H0.
+Qed.
+
+Lemma eqmaybe_semiprivate_not_bot' : forall (A : Ty) l (x y : [Option A]), l <> \bot -> rel (eqmaybe (semiprivateRel _)) l x y -> x = y.
+Proof.
+ssa. de x. de y. de H0. subst. done. de y.
+Qed.
+
+Lemma eqmaybe_public_not_bot : forall (A : Ty) l (x y : [Option A]), l <> \bot -> rel (eqmaybe (publicRel _)) l x y -> x = y.
+Proof.
+ssa. de x. de y. subst. done. de y.
+Qed.
+
+Lemma eqmaybe_semiprivate_not_bot : forall (A : Ty) l (x y : [Option A]), l <> \bot -> rel (eqmaybe_top (semiprivateRel _)) l x y -> x = y.
+Proof.
+ssa. de x. de y. de H0. subst. done. de y.
+Qed.
+
+Lemma eqmaybe_semiprivate_bot : forall (A : Ty) (x y : [Option A]), rel (eqmaybe_top (semiprivateRel _)) \bot x y.
+Proof.
+  ssa. de x. de y. de y.
+Qed.
+
+Lemma semiprivate_bot : forall (A : Ty) (x y : [A]), rel ((semiprivateRel _)) \bot x y.
+Proof.
+  ssa.
+Qed.
+
+Hint Resolve semiprivate_bot.
+
+Lemma publicRel_eq : forall (A : Ty) l x y, rel (publicRel A) l x y -> x = y.
+Proof. ssa. Qed.
+
+Lemma out_rel_not_bot : forall i i' l, l <> \bot -> rel out_rel l i i' -> i = i'.
+Proof.
+  intros.
+  move:H0. move/rel_eqpair=> [] + /rel_eqpair [] + /rel_eqpair [] + /rel_eqpair [] + /rel_eqpair [].
+  move: i=>[a [b [c [d [e f]]]]].
+  move: i'=>[a' [b' [c' [d' [e' f']]]]].  
+  rewrite !pair_rewr.
+  move=>/eqmaybe_public_not_bot=>->//.
+  move=>/eqmaybe_semiprivate_not_bot'=>->//.
+  move=>/eqmaybe_public_not_bot=>->//.
+  move/rel_eqmaybe_top.
+  case.
+  move=>[x0][y0][]->[]-> /semiprivate_not_bot' ->//.
+  move=>/eqmaybe_semiprivate_not_bot=>->//.
+  move=>/eqmaybe_public_not_bot=>->//.
+  case. ssa.
+  case. ssa.
+  move=>[]->->.
+  move=>/eqmaybe_semiprivate_not_bot=>->//.
+  move=>/eqmaybe_public_not_bot=>->//.  
+Qed.
+
+
+
+Lemma falseRel_aware : forall l, aware falseRel true l.
+Proof.
+intros. rewrite /aware. intros. ssa. subst. simpl. intro. ssa.
+Qed.
+
+Definition pids_rel : myrel [pids] := eqpair (eqsum (semiprivateRel _) (publicRel _)) (publicRel _).
+Definition hidden_pending : myrel [I_bits] := eqpair (semiprivateRel _) (publicRel _).
+Definition public_pair : myrel [I_bits] := eqpair (publicRel _) (publicRel _).
+Definition ic_rel : myrel [ic] := eqpair hidden_pending (eqpair hidden_pending public_pair).
+Definition bool_state_rel : myrel [bool_state] := eqpair (publicRel _) (eqpair (publicRel _) ic_rel).
+Definition stateType_rel : myrel [stateType] := eqpair pids_rel bool_state_rel.
+
+
+Lemma stateType_rel_not_bot : forall i i' l, l <> \bot -> rel stateType_rel l i i' -> i = i'.
+Proof.
+  intros.
+  move:H0.
+  move/rel_eqpair=> [] /rel_eqpair[] + + /rel_eqpair [] + /rel_eqpair [] + /rel_eqpair [] /rel_eqpair [] + + /rel_eqpair[] /rel_eqpair[] + + /rel_eqpair [] + +.
+  move: i=>[[a0 a1]] [b [b0 [[b1 b2 [[b3 b4 [b5 b6]]]]]]].
+  move: i'=>[[a0' a1']] [b' [b0' [[b1' b2' [[b3' b4' [b5' b6']]]]]]].  
+  rewrite !pair_rewr. 
+  move=> /eqsum_split Hsplit.
+  move=>/publicRel_eq -> /publicRel_eq -> /publicRel_eq -> // /semiprivate_not_bot' -> // /publicRel_eq -> // /semiprivate_not_bot' -> // /publicRel_eq -> // /publicRel_eq -> /publicRel_eq ->.
+  case: Hsplit.
+  move=>[x][y][]->[]->/semiprivate_not_bot' ->//.
+  move=>[x][y][]->[]-> /publicRel_eq ->//.  
+Qed.
+
+
+Transparent state_step f_si initial_state def f_proj.
+
+Lemma in_rel_eq i i0 l : rel in_rel l i i0 -> i = i0.
+Proof.
+  ssa. de H. move: H H0. rewrite /ir_dis. ssa. subst. done.
+Qed.
+
+Lemma sta_comp : forall (I V O : Ty) (IRel : myrel [I]) (VRel : myrel [V]) (ORel : myrel [O]) (f f' : [I] -> [V] -> [V]) (g : [O] -> [V] -> [V])
+                        (v : [V]) (p : Proc (Times V I) O),
+    fv_NI ORel VRel VRel g ->
+    fv_NI IRel VRel VRel f -> f_EP IRel VRel f ->
+    fv_NI IRel VRel VRel f' -> f_EP IRel VRel f' ->
+    NI (eqpair_R VRel IRel) ORel p ->    
+    NI IRel (eqpair VRel ORel) (sta (fun i => (f i) \o (f' i)) g v p).
+Proof.
+  intros.
+  apply sta_NI;eauto.
+  move: H0 H2. clear.
+  rewrite /fv_NI. intros. eauto.
+  move: H1 H3. clear.
+  rewrite /f_EP. intros. eauto.
+Qed.
+
+
+Lemma fv_NI_comp : forall (I V: Ty) (IRel : myrel [I]) (VRel : myrel [V]) (f f' : [I]  -> [V] ->  [V]),
+    fv_NI IRel VRel VRel f -> fv_NI IRel VRel VRel f' -> fv_NI IRel VRel VRel (fun i => (f' i) \o (f i)).
+Proof.
+intros. move: H H0. rewrite /fv_NI. ssa.
+Qed.
+Check f_EP.
+Lemma f_EP_comp : forall (I V: Ty) (IRel : myrel [I]) (VRel : myrel [V]) (f f' : [I]  -> [V] ->  [V]),
+    f_EP IRel VRel f -> f_EP IRel VRel f' -> f_EP IRel VRel (fun i => (f' i) \o (f i)).
+Proof.
+intros. move: H H0. rewrite /f_EP. ssa. eauto.
+Qed.
+
+Lemma fv_NI_step_left : forall f,
+    fv_NI in_rel stateType_rel stateType_rel f -> fv_NI (eqsum in_rel out_rel) stateType_rel stateType_rel (step_left f).
+Proof.
+  ssa. move: H. mrw. intros.
+  apply eqsum_llrr in H0 as H0'. destruct H0'. destruct H2. destruct i. destruct i'.
+  rewrite /step_left. eauto. done. done.
+  destruct H2. destruct i. done. destruct i'. done.
+  rewrite /step_left. eauto.
+Qed.
+
+Lemma fv_NI_step_right : forall f,
+    fv_NI out_rel stateType_rel stateType_rel f -> fv_NI (eqsum in_rel out_rel) stateType_rel stateType_rel (step_right f).
+Proof.
+  ssa. move: H. mrw. intros.
+  apply eqsum_llrr in H0 as H0'. destruct H0'. destruct H2. destruct i. destruct i'.
+  rewrite /step_left. eauto. done. done.
+  destruct H2. destruct i. done. destruct i'. done.
+  rewrite /step_left. eauto.
+Qed.
+
+Lemma f_EP_left : forall f,
+    f_EP in_rel stateType_rel f -> f_EP (eqsum in_rel out_rel) stateType_rel (step_left f).
+Proof.
+  ssa.
+Qed.
+
+Lemma f_EP_right : forall f,
+    f_EP out_rel stateType_rel f -> f_EP (eqsum in_rel out_rel) stateType_rel (step_right f).
+Proof.
+  ssa.
+Qed.
+
+Definition ready_aux (v : [stateType]) := I_ready v TimerInterrupt /\ first_ready v = Some TimerInterrupt \/ ~ I_ready v TimerInterrupt /\ I_ready v DiskInterrupt /\ first_ready v = Some DiskInterrupt \/  ~ I_ready v TimerInterrupt /\ ~ I_ready v DiskInterrupt /\ I_ready v DefaultInterrupt /\ first_ready v = Some DefaultInterrupt \/ ~ I_ready v TimerInterrupt /\ ~ I_ready v DiskInterrupt /\ ~ I_ready v DefaultInterrupt /\ first_ready v = None.
+
+Lemma ready_auxP v : ready_aux v.
+Proof.
+  rewrite /ready_aux.
+  destruct (I_ready v TimerInterrupt) eqn:Heqn. left. ssa.
+  rewrite /first_ready. rewrite /all_interrupts /ohead. rewrite /filter.
+  rewrite Heqn. done.
+  right.
+  destruct (I_ready v DiskInterrupt) eqn:Heqn'.
+  left. con. done. con. done.
+  rewrite /first_ready /ohead /filter /all_interrupts Heqn Heqn' //.
+  right.
+  destruct (I_ready v DefaultInterrupt) eqn:Heqn''.
+  left. con. done. con. done. con. done.
+  rewrite /first_ready /ohead /filter /all_interrupts Heqn Heqn' Heqn''//.
+  rewrite /first_ready /ohead /filter /all_interrupts Heqn Heqn' Heqn''//. ssa.
+Qed.
+
+
+Definition ready_cases (v v' : [stateType]) := ready_aux v /\ ready_aux v'.
+
+Definition ready_aux2 (v : [stateType]) := I_ready v DiskInterrupt /\ first_ready v = Some DiskInterrupt \/
+                                             ~ I_ready v DiskInterrupt /\ I_ready v DefaultInterrupt /\ first_ready v = Some DefaultInterrupt \/
+                                             ~ I_ready v DiskInterrupt /\ ~ I_ready v DefaultInterrupt /\ first_ready v = None.
+
+Definition ready_cases2 (v v' : [stateType]) := I_ready v TimerInterrupt /\ I_ready v' TimerInterrupt /\ first_ready v = Some TimerInterrupt /\ first_ready v' = Some TimerInterrupt \/
+                                                  ~ I_ready v TimerInterrupt /\ ~ I_ready v' TimerInterrupt /\
+                                                    ready_aux2 v /\ ready_aux2 v'.
+
+Lemma ready_casesP v v' : ready_cases v v'.
+Proof.
+  rewrite /ready_cases. con. apply ready_auxP. apply ready_auxP.
+Qed.
+
+Lemma ready_cases2P v v' : I_ready v TimerInterrupt = I_ready v' TimerInterrupt -> ready_cases2 v v'.
+Proof.
+  rewrite /ready_cases2.
+  move: (ready_casesP v v'). rewrite /ready_cases. case.
+  rewrite /ready_aux. intros. rewrite H in a b. rewrite H.
+  de a. de b.
+  de H2. de H2. de H0. de b. de H3. right. ssa. rewrite /ready_aux2. ssa. rewrite /ready_aux2. ssa.
+  de H3. right. ssa.
+  rewrite /ready_aux2;ssa.
+  rewrite /ready_aux2;ssa.
+  right. ssa.
+  rewrite /ready_aux2;ssa.
+  rewrite /ready_aux2;ssa.
+  de H0.
+  de b. de H4.
+  right. ssa.
+  rewrite /ready_aux2;ssa.
+  rewrite /ready_aux2;ssa.
+  de H4.
+  right.
+  ssa.
+  rewrite /ready_aux2;ssa.
+  rewrite /ready_aux2;ssa.
+  right.
+  ssa; rewrite /ready_aux2;ssa.
+  de b. de H4.
+  right;  rewrite /ready_aux2;ssa.
+  de H4.
+  right;  rewrite /ready_aux2;ssa.
+  right;  rewrite /ready_aux2;ssa.
+Qed.
+
+Lemma first_ready_update_re_sch : forall v b, first_ready (update_re_sch v b) = first_ready v.
+Proof.
+  intros. cbv. ssa.
+Qed.
+
+Lemma model_good_NI : NI in_rel out_rel model_good.
+Proof.
+  rewr;simpl;rewr;simpl.
+  eapply map_NI.
+  instantiate (1:= eqsum_L in_rel out_rel). ssa. ssa.
+  mrw. intros.
+  2:eapply loop_NI. apply eqsum_L_llrr in H as H'. destruct H'.
+  destruct i. destruct i'. ssa. ssa. ssa.
+  destruct i. ssa. destruct i'. ssa.
+  apply rel_eqsum_L2' in H. 
+  rewrite /inr_or_def. done.
+
+  eapply map_NI.
+  eauto. eauto.
+  mrw. intros.
+  case/rel_eqpair: H;eauto.
+  instantiate (1:= stateType_rel).
+
+  (*state update: This part is long. Involves step0, step1, step2*)
+  apply sta_NI.
+  mrw;eauto.
+
+  apply fv_NI_comp.
+
+  (*step0*)
+  rewrite /step0.
+  apply fv_NI_step_left.
+
+  mrw. intros.
+  apply in_rel_eq in H;subst.
+  move: H0.
+  move/rel_eqpair=>[H0] /rel_eqpair[H1] /rel_eqpair[]H2 /rel_eqpair[]/rel_eqpair[]H3 H4/rel_eqpair[]/rel_eqpair[]H5 H6/rel_eqpair[]H7 H8.
+  move: H0 H1 H2 H3 H4 H5 H6 H7 H8.
+  move: v=> [[cur prev]] [re_sch] [ir_count] [[def_pending def_mask]] [[disk_pending disk_mask]] [timer_pending timer_mask].
+  move: v'=> [[cur' prev']] [re_sch'] [ir_count'] [[def_pending' def_mask']] [[disk_pending' disk_mask']] [timer_pending' timer_mask'].
+  rewrite /get_ic /update_ic /get_bool_state /update_bool_state /get_I_mask /get_mask' /update_I_pending /update_I_bits /update_I_bits' !pair_rewr.
+  move=> H0 H1 H2 H3 H4 H5 H6 H7 H8.
+  rewrite /get_ic /update_ic /get_bool_state /update_bool_state /get_I_mask /get_mask' /update_I_pending /update_I_bits /update_I_bits' !pair_rewr.    
+
+  apply/rel_eqpair2;con;first ssa.
+  apply/rel_eqpair2;con;first ssa.
+  apply/rel_eqpair2.
+  rewrite !pair_rewr.
+  con. done.
+  apply/rel_eqpair2;con. 
+  apply/rel_eqpair2;con.
+
+  destruct i';rewrite !pair_rewr;eauto.
+  destruct i';rewrite !pair_rewr;eauto.
+  apply/rel_eqpair2;con.
+  apply/rel_eqpair2;con.  
+  destruct i';rewrite !pair_rewr //.
+  destruct i';rewrite !pair_rewr //.
+  destruct i';rewrite !pair_rewr //.    
+
+  apply fv_NI_comp.
+
+  (*step1*)
+  rewrite /step1.
+  apply fv_NI_step_right. rewrite /check_scheduler.
+
+  mrw. intros.
+
+  destruct (eqVneq l \bot).
+  2: {  apply out_rel_not_bot in H. 2:apply/eqP=>//. subst.
+        apply stateType_rel_not_bot in H0. 2:apply/eqP=>//. subst. eauto. }
+  subst.  
+
+  move: v H0=> [[cur prev]] [re_sch] [ir_count] [[def_pending def_mask]] [[disk_pending disk_mask]] [timer_pending timer_mask].
+  move: v'=> [[cur' prev']] [re_sch'] [ir_count'] [[def_pending' def_mask']] [[disk_pending' disk_mask']] [timer_pending' timer_mask'].  
+
+  move/rel_eqpair=>[H0] /rel_eqpair[H1] /rel_eqpair[] /publicRel_eq H2 /rel_eqpair[]/rel_eqpair[H3 H4] /rel_eqpair[] H5 H6. 
+  rewrite !pair_rewr in H0 H1 H2 H3 H4 H5 H6.
+
+  move: H=> /rel_eqpair[] + /rel_eqpair[] + /rel_eqpair[] + /rel_eqpair[] _ /rel_eqpair[] _ +.
+  move: i=>[a[] b[] c[] d[] e f].
+  move: i'=>[a'[] b'[] c'[] d'[] e' f']. 
+  rewrite !pair_rewr /is_sch_out. subst.
+ 
+  case/rel_eqmaybe2.
+  move=>[]x []y []-> []->// /publicRel_eq ->//.
+  move=>[]->[]->//.
+
+  case/rel_eqmaybe2.
+  move=>[]x' []y' []-> []->// Hpr.
+  move=>[]->[]->//.
+
+  case/rel_eqmaybe2.
+  move=>[]x0 []y0 []-> []->// /publicRel_eq ->//.
+
+  move=>_. (*drop*)
+
+  apply/rel_eqpair2;con;try solve [ssa].
+
+  move=>[]->[]->//.
+
+
+  (*step1*)
+  apply fv_NI_comp.
+  
+  apply fv_NI_step_right.
+
+  apply fv_NI_comp.
+
+  mrw. intros.
+  rewrite /initiate_ir.
+
+  have: tI_out i = tI_out i'.
+
+  move: v H0=> [[cur prev]] [re_sch] [ir_count] [[def_pending def_mask]] [[disk_pending disk_mask]] [timer_pending timer_mask].
+  move: v'=> [[cur' prev']] [re_sch'] [ir_count'] [[def_pending' def_mask']] [[disk_pending' disk_mask']] [timer_pending' timer_mask'].  
+
+  move/rel_eqpair=>[H0] /rel_eqpair[H1] /rel_eqpair[] H2 /rel_eqpair[]/rel_eqpair[H3 H4] /rel_eqpair[] H5 H6.
+  rewrite !pair_rewr in H0 H1 H2 H3 H4 H5 H6.
+
+  move: H=> /rel_eqpair[] _ /rel_eqpair[] _ /rel_eqpair[] _ /rel_eqpair[] _ /rel_eqpair[] _ +.
+  move: i=>[a[] b[] c[] d[] e f].
+  move: i'=>[a'[] b'[] c'[] d'[] e' f']. 
+  rewrite !pair_rewr /is_sch_out.  
+
+  case/rel_eqmaybe2.
+  move=>[]x'[]y'[]->[]->/publicRel_eq->//.
+  move=>[]->->//.
+
+  move=>->.
+
+  destruct ((tI_out i')). destruct h. done.
+  apply/rel_eqpair2. con;ssa. done.
+
+
+  apply fv_NI_comp.
+  mrw. intros.
+  rewrite /check_handler_completed.
+
+  have: get_ir_count v = get_ir_count v'.
+
+  move: v H0=> [[cur prev]] [re_sch] [ir_count] [[def_pending def_mask]] [[disk_pending disk_mask]] [timer_pending timer_mask].
+  move: v'=> [[cur' prev']] [re_sch'] [ir_count'] [[def_pending' def_mask']] [[disk_pending' disk_mask']] [timer_pending' timer_mask'].  
+
+  move/rel_eqpair=>[H0] /rel_eqpair[H1] /rel_eqpair[] H2 /rel_eqpair[]/rel_eqpair[H3 H4] /rel_eqpair[] H5 H6.
+  rewrite !pair_rewr in H0 H1 H2 H3 H4 H5 H6.
+
+  move: H2=>/publicRel_eq->//.
+  move=>->.
+  destruct (handler_completed (get_ir_count v')).
+
+  apply/rel_eqpair2. con. ssa.
+  apply/rel_eqpair2. con. ssa.  
+  apply/rel_eqpair2. con. ssa.
+  apply/rel_eqpair2. con. 
+  apply/rel_eqpair2. con. ssa. eauto.
+  apply/rel_eqpair2. con.
+  apply/rel_eqpair2. con. ssa. eauto.
+  apply/rel_eqpair2. con. ssa. ssa. done.
+
+  mrw. intros.
+  rewrite /check_ir_count.
+
+  have: get_ir_count v = get_ir_count v'.
+
+  move: v H0=> [[cur prev]] [re_sch] [ir_count] [[def_pending def_mask]] [[disk_pending disk_mask]] [timer_pending timer_mask].
+  move: v'=> [[cur' prev']] [re_sch'] [ir_count'] [[def_pending' def_mask']] [[disk_pending' disk_mask']] [timer_pending' timer_mask'].  
+
+  move/rel_eqpair=>[H0] /rel_eqpair[H1] /rel_eqpair[] H2 /rel_eqpair[]/rel_eqpair[H3 H4] /rel_eqpair[] H5 H6.
+  rewrite !pair_rewr in H0 H1 H2 H3 H4 H5 H6.
+
+  move: H2=>/publicRel_eq->//.
+  move=>->.
+
+  destruct (get_ir_count v').
+  destruct n.
+
+  apply/rel_eqpair2. con. ssa.
+  apply/rel_eqpair2. con. ssa.  
+  apply/rel_eqpair2. con. ssa.
+  apply/rel_eqpair2. con. 
+  apply/rel_eqpair2. con. ssa. eauto.
+  apply/rel_eqpair2. con.
+  apply/rel_eqpair2. con. ssa. eauto.
+  apply/rel_eqpair2. con. ssa. ssa.
+
+  apply/rel_eqpair2. con. ssa.
+  apply/rel_eqpair2. con. ssa.  
+  apply/rel_eqpair2. con. ssa.
+  apply/rel_eqpair2. con. 
+  apply/rel_eqpair2. con. ssa.
+
+  move: v H0=> [[cur prev]] [re_sch] [ir_count] [[def_pending def_mask]] [[disk_pending disk_mask]] [timer_pending timer_mask].
+  move: v'=> [[cur' prev']] [re_sch'] [ir_count'] [[def_pending' def_mask']] [[disk_pending' disk_mask']] [timer_pending' timer_mask'].    rewrite !pair_rewr.
+
+  move/rel_eqpair=>[H0] /rel_eqpair[H1] /rel_eqpair[] H2 /rel_eqpair[]/rel_eqpair[H3 H4] /rel_eqpair[] H5 H6.
+  rewrite !pair_rewr in H0 H1 H2 H3 H4 H5 H6. eauto.
+  
+  apply/rel_eqpair2. con. ssa.
+  apply/rel_eqpair2. con. ssa. ssa. done.
+
+  mrw. intros.
+  destruct (eqVneq l \bot).
+  2: { move/eqsum_split : H. case.
+       move=>[]x[]y[]->[]->. ssa.
+       move=>[]x[]y[]->[]->. 
+       apply stateType_rel_not_bot in H0. 2:apply/eqP=>//. subst. eauto.
+  }
+
+  subst.
+
+  move/eqsum_split: H. case.
+  move=>[]x[]y[]->[]->. ssa.
+  move=>[]x[]y[]->[]->. move=>Hout.
+  rewrite /step_right.
+
+  rewrite /initiate_next.
+
+  have: masks_set v = masks_set v'.
+
+  move: v H0=> [[cur prev]] [re_sch] [ir_count] [[def_pending def_mask]] [[disk_pending disk_mask]] [timer_pending timer_mask].
+  move: v'=> [[cur' prev']] [re_sch'] [ir_count'] [[def_pending' def_mask']] [[disk_pending' disk_mask']] [timer_pending' timer_mask']. 
+
+  move/rel_eqpair=>[H0] /rel_eqpair[H1] /rel_eqpair[] H2 /rel_eqpair[]/rel_eqpair[H3 H4] /rel_eqpair[] H5 H6.
+  rewrite !pair_rewr in H0 H1 H2 H3 H4 H5 H6.
+
+  move: H4 H5 H6.
+  move=>/publicRel_eq ->.
+  move=>/rel_eqpair[] _. rewrite !pair_rewr=> /publicRel_eq ->.
+  move=>/rel_eqpair[] _. rewrite !pair_rewr=> /publicRel_eq ->. ssa.
+  move=>->.
+  
+  destruct (masks_set v'). done. 
+
+  have: I_ready  (bool_coding v) TimerInterrupt =
+          I_ready (bool_coding v') TimerInterrupt. 
+
+
+  move: v H0=> [[cur prev]] [re_sch] [ir_count] [[def_pending def_mask]] [[disk_pending disk_mask]] [timer_pending timer_mask].
+  move: v'=> [[cur' prev']] [re_sch'] [ir_count'] [[def_pending' def_mask']] [[disk_pending' disk_mask']] [timer_pending' timer_mask'].  
+
+  move/rel_eqpair=>[H0] /rel_eqpair[H1] /rel_eqpair[] H2 /rel_eqpair[]/rel_eqpair[H3 H4] /rel_eqpair[] H5 H6.
+  rewrite !pair_rewr in H0 H1 H2 H3 H4 H5 H6.
+
+  move: H6. move/rel_eqpair=>[]. rewrite !pair_rewr. move=>/publicRel_eq->/publicRel_eq->.
+  move/publicRel_eq : H2=>->//. 
+  
+  move/ready_cases2P. rewrite /ready_cases2.
+
+  move=>[[]Hready[]Hready'[]Hfirst Hfirst'|[]Hready[]Hready'[]Haux Haux'].
+  rewrite Hfirst Hfirst'.
+
+  clear Hready Hready' Hfirst Hfirst'.
+
+  move: v H0=> [[cur prev]] [re_sch] [ir_count] [[def_pending def_mask]] [[disk_pending disk_mask]] [timer_pending timer_mask].
+  move: v'=> [[cur' prev']] [re_sch'] [ir_count'] [[def_pending' def_mask']] [[disk_pending' disk_mask']] [timer_pending' timer_mask'].    
+  move/rel_eqpair=>[H0] /rel_eqpair[H1] /rel_eqpair[] H2 /rel_eqpair[]/rel_eqpair[H3 H4] /rel_eqpair[] H5 H6.
+  rewrite !pair_rewr in H0 H1 H2 H3 H4 H5 H6.  
+
+  apply/rel_eqpair2. con.
+  apply/rel_eqpair2. con.
+  rewrite /initiate_handler !pair_rewr. ssa.
+
+  move/rel_eqpair2 : H0=>[]. rewrite !pair_rewr.
+  move/eqsum_split.
+  case.
+  move=>[]i0'[]i1'[]->[]->_/publicRel_eq ->. rewrite !pair_rewr //.
+  move=>[]i0'[]i1'[]->[]->/publicRel_eq ->/publicRel_eq ->. rewrite !pair_rewr //.
+  apply/rel_eqpair2. con.
+
+  move/rel_eqpair2 : H0=>[]. rewrite !pair_rewr.
+  move/eqsum_split.
+  case.
+  move=>[]i0'[]i1'[]->[]->_/publicRel_eq ->. rewrite !pair_rewr //.
+  move/publicRel_eq : H1=>->//.
+  move=>[]i0'[]i1'[]->[]->/publicRel_eq ->/publicRel_eq ->. rewrite !pair_rewr //.
+  move/publicRel_eq : H1=>->//.  
+  apply/rel_eqpair2. con.
+
+  move/rel_eqpair2 : H0=>[]. rewrite !pair_rewr.
+  move/eqsum_split.
+  case.
+  move=>[]i0'[]i1'[]->[]->_/publicRel_eq ->. rewrite !pair_rewr //.
+  move/publicRel_eq : H1=>->//.
+  move=>[]i0'[]i1'[]->[]->/publicRel_eq ->/publicRel_eq ->. rewrite !pair_rewr //.
+  move/publicRel_eq : H1=>->//.  
+  
+  move:Haux Haux'.
+  rewrite /ready_aux2.
+  move=>[[]HreadyD Hfirst|].
+  move=>[[]HreadyD' Hfirst'|[]].
+  rewrite Hfirst Hfirst'.
+
+
+  clear Hready Hready' Hfirst Hfirst' HreadyD HreadyD'.
+
+  move: v H0=> [[cur prev]] [re_sch] [ir_count] [[def_pending def_mask]] [[disk_pending disk_mask]] [timer_pending timer_mask].
+  move: v'=> [[cur' prev']] [re_sch'] [ir_count'] [[def_pending' def_mask']] [[disk_pending' disk_mask']] [timer_pending' timer_mask'].    
+  move/rel_eqpair=>[H0] /rel_eqpair[H1] /rel_eqpair[] H2 /rel_eqpair[]/rel_eqpair[H3 H4] /rel_eqpair[] H5 H6.
+  rewrite !pair_rewr in H0 H1 H2 H3 H4 H5 H6.  
+
+  apply/rel_eqpair2. con.
+  apply/rel_eqpair2. con.
+  rewrite /initiate_handler !pair_rewr. ssa. 
+
+  move/rel_eqpair2 : H0=>[]. rewrite !pair_rewr.
+  move/eqsum_split.
+  case.
+  move=>[]i0'[]i1'[]->[]->_/publicRel_eq ->. rewrite !pair_rewr //.
+  move=>[]i0'[]i1'[]->[]->/publicRel_eq ->/publicRel_eq ->. rewrite !pair_rewr //.
+  apply/rel_eqpair2. con.
+
+  move/publicRel_eq : H2=>->.
+  move/rel_eqpair2 : H0=>[]. rewrite !pair_rewr.
+  move/eqsum_split.
+  case.
+  move=>[]i0'[]i1'[]->[]->_/publicRel_eq ->. rewrite !pair_rewr //.
+  move/publicRel_eq : H1=>->//.
+  move=>[]i0'[]i1'[]->[]->/publicRel_eq ->/publicRel_eq ->. rewrite !pair_rewr //.
+  move/publicRel_eq : H1=>->//.  
+  apply/rel_eqpair2. con.
+
+  move/rel_eqpair2 : H0=>[]. rewrite !pair_rewr.
+  move/eqsum_split.
+  case.
+  move=>[]i0'[]i1'[]->[]->_/publicRel_eq ->. rewrite !pair_rewr //.
+  move/publicRel_eq : H1=>->//.
+  move=>[]i0'[]i1'[]->[]->/publicRel_eq ->/publicRel_eq ->. rewrite !pair_rewr //.
+
+  apply/rel_eqpair2. con.
+  apply/rel_eqpair2. con. eauto. ssa.
+  apply/rel_eqpair2. con.
+  apply/rel_eqpair2. con. eauto. ssa.
+  apply/rel_eqpair2. con.
+
+  move/rel_eqpair2 : H6. case. rewrite !pair_rewr. move=>/publicRel_eq->//. 
+  move/rel_eqpair2 : H0=>[]. rewrite !pair_rewr.
+  move/eqsum_split.
+  case.
+  move=>[]i0'[]i1'[]->[]->_/publicRel_eq ->//. 
+  move=>[]i0'[]i1'[]->[]-> /publicRel_eq ->/publicRel_eq ->. ssa.
+
+  move/publicRel_eq : H4=>->//.
+
+  move=>[]HreadyD'[]HreadyDef' Hfirst'.
+  rewrite Hfirst Hfirst'.
+
+  clear Hready Hready' Hfirst Hfirst' HreadyD HreadyD' HreadyDef'.
+
+  move: v H0=> [[cur prev]] [re_sch] [ir_count] [[def_pending def_mask]] [[disk_pending disk_mask]] [timer_pending timer_mask].
+  move: v'=> [[cur' prev']] [re_sch'] [ir_count'] [[def_pending' def_mask']] [[disk_pending' disk_mask']] [timer_pending' timer_mask'].    
+  move/rel_eqpair=>[H0] /rel_eqpair[H1] /rel_eqpair[] H2 /rel_eqpair[]/rel_eqpair[H3 H4] /rel_eqpair[] H5 H6.
+  rewrite !pair_rewr in H0 H1 H2 H3 H4 H5 H6.  
+
+  apply/rel_eqpair2. con.
+  apply/rel_eqpair2. con.
+  rewrite /initiate_handler !pair_rewr. ssa. 
+
+  move/rel_eqpair2 : H0=>[]. rewrite !pair_rewr.
+  move/eqsum_split.
+  case.
+  move=>[]i0'[]i1'[]->[]->_/publicRel_eq ->. rewrite !pair_rewr //.
+  move=>[]i0'[]i1'[]->[]->/publicRel_eq ->/publicRel_eq ->. rewrite !pair_rewr //.
+  apply/rel_eqpair2. con.
+
+  move/publicRel_eq : H2=>->.
+  move/rel_eqpair2 : H0=>[]. rewrite !pair_rewr.
+  move/eqsum_split.
+  case.
+  move=>[]i0'[]i1'[]->[]->_/publicRel_eq ->. rewrite !pair_rewr //.
+  move/publicRel_eq : H1=>->//.
+  move=>[]i0'[]i1'[]->[]->/publicRel_eq ->/publicRel_eq ->. rewrite !pair_rewr //.
+  move/publicRel_eq : H1=>->//.  
+  apply/rel_eqpair2. con.
+
+  move/rel_eqpair2 : H0=>[]. rewrite !pair_rewr.
+  move/eqsum_split.
+  case.
+  move=>[]i0'[]i1'[]->[]->_/publicRel_eq ->. rewrite !pair_rewr //.
+  move/publicRel_eq : H1=>->//.
+  move=>[]i0'[]i1'[]->[]->/publicRel_eq ->/publicRel_eq ->. rewrite !pair_rewr //.
+
+  apply/rel_eqpair2. con.
+  apply/rel_eqpair2. con. eauto. ssa.
+  apply/rel_eqpair2. con.
+  apply/rel_eqpair2. con. eauto. ssa.
+  apply/rel_eqpair2. con.
+
+  move/rel_eqpair2 : H6. case. rewrite !pair_rewr. move=>/publicRel_eq->//. 
+  move/rel_eqpair2 : H0=>[]. rewrite !pair_rewr.
+  move/eqsum_split.
+  case.
+  move=>[]i0'[]i1'[]->[]->_/publicRel_eq ->//. 
+  move=>[]i0'[]i1'[]->[]-> /publicRel_eq ->/publicRel_eq ->. ssa.
+
+  move/publicRel_eq : H4=>->//.
+
+
+  move=>[]HreadyD'[]HreadyDef' Hfirst'.
+  rewrite Hfirst Hfirst'. exfalso.
+  clear Hready Hready' Hfirst Hfirst'.
+  
+  move: v H0 HreadyD HreadyD' HreadyDef'=> [[cur prev]] [re_sch] [ir_count] [[def_pending def_mask]] [[disk_pending disk_mask]] [timer_pending timer_mask].
+  move: v'=> [[cur' prev']] [re_sch'] [ir_count'] [[def_pending' def_mask']] [[disk_pending' disk_mask']] [timer_pending' timer_mask'].    
+  move/rel_eqpair=>[_] /rel_eqpair[_] /rel_eqpair[] HH /rel_eqpair[]/rel_eqpair[_ H4] /rel_eqpair[] /rel_eqpair[] _ H5 /rel_eqpair[] _ H6.
+  rewrite !pair_rewr in HH H4 H5 H6.  
+  move: HH H4 H5 H6. move=>/publicRel_eq->/publicRel_eq->/publicRel_eq->/publicRel_eq->. 
+
+  rewrite /I_ready /get_I_pending /get_pending' /get_I_bits /get_I_bits' /get_ic /get_ic_count /get_bool_state /bool_coding /get_I_mask /get_mask' /get_I_bits /get_I_bits' /get_ic /get_ic_count /get_bool_state /update_bool_state !pair_rewr /timeslice_live /get_ir_count /get_ic_count /get_bool_state !pair_rewr.
+  move=>+ /negP + /negP.
+  rewrite !negb_and !negbK.
+  move/andP. case.
+  rewrite orbC [ false || _ ]/orb.
+  move=>Hpending.
+  rewrite !negb_or !negbK.
+  move/andP. case. move=>Hmask Hir.
+  move/orP. case.
+  simpl. move/orP. case.
+  move=>HH. move/orP. case.
+  move/andP. ssa. ssa. apply/negP. apply H0. done. 
+  move/orP. case. intro. apply/negP. apply Hmask. done.
+  intro. apply/negP. apply b. done. done.
+  move/orP. case. intro. rewrite a in Hmask. done.
+  rewrite Hir. done.
+
+  move=>[[]HreadyD[]HreadyDef Hfirst|].
+  move=>[[]HreadyD' Hfirst'|].
+  rewrite Hfirst Hfirst'.
+
+  clear Hready Hready' Hfirst Hfirst' HreadyD HreadyD' HreadyDef.
+
+  move: v H0=> [[cur prev]] [re_sch] [ir_count] [[def_pending def_mask]] [[disk_pending disk_mask]] [timer_pending timer_mask].
+  move: v'=> [[cur' prev']] [re_sch'] [ir_count'] [[def_pending' def_mask']] [[disk_pending' disk_mask']] [timer_pending' timer_mask'].    
+  move/rel_eqpair=>[H0] /rel_eqpair[H1] /rel_eqpair[] H2 /rel_eqpair[]/rel_eqpair[H3 H4] /rel_eqpair[] H5 H6.
+  rewrite !pair_rewr in H0 H1 H2 H3 H4 H5 H6.  
+
+  apply/rel_eqpair2. con.
+  apply/rel_eqpair2. con.
+  rewrite /initiate_handler !pair_rewr. ssa. 
+
+  move/rel_eqpair2 : H0=>[]. rewrite !pair_rewr.
+  move/eqsum_split.
+  case.
+  move=>[]i0'[]i1'[]->[]->_/publicRel_eq ->. rewrite !pair_rewr //.
+  move=>[]i0'[]i1'[]->[]->/publicRel_eq ->/publicRel_eq ->. rewrite !pair_rewr //.
+  apply/rel_eqpair2. con.
+
+  move/publicRel_eq : H2=>->.
+  move/rel_eqpair2 : H0=>[]. rewrite !pair_rewr.
+  move/eqsum_split.
+  case.
+  move=>[]i0'[]i1'[]->[]->_/publicRel_eq ->. rewrite !pair_rewr //.
+  move/publicRel_eq : H1=>->//.
+  move=>[]i0'[]i1'[]->[]->/publicRel_eq ->/publicRel_eq ->. rewrite !pair_rewr //.
+  move/publicRel_eq : H1=>->//.  
+  apply/rel_eqpair2. con.
+
+  move/rel_eqpair2 : H0=>[]. rewrite !pair_rewr.
+  move/eqsum_split.
+  case.
+  move=>[]i0'[]i1'[]->[]->_/publicRel_eq ->. rewrite !pair_rewr //.
+  move/publicRel_eq : H1=>->//.
+  move=>[]i0'[]i1'[]->[]->/publicRel_eq ->/publicRel_eq ->. rewrite !pair_rewr //.
+
+  apply/rel_eqpair2. con.
+  apply/rel_eqpair2. con. eauto. ssa.
+  apply/rel_eqpair2. con.
+  apply/rel_eqpair2. con. eauto. ssa.
+  apply/rel_eqpair2. con.
+
+  move/rel_eqpair2 : H6. case. rewrite !pair_rewr. move=>/publicRel_eq->//. 
+  move/rel_eqpair2 : H0=>[]. rewrite !pair_rewr.
+  move/eqsum_split.
+  case.
+  move=>[]i0'[]i1'[]->[]->_/publicRel_eq ->//. 
+  move=>[]i0'[]i1'[]->[]-> /publicRel_eq ->/publicRel_eq ->. ssa.
+
+  move/publicRel_eq : H4=>->//.  
+  
+
+  move=>[[]HreadyD'[]HreadyDef' Hfirst'|].
+  rewrite Hfirst Hfirst'.
+
+  clear Hready Hready' Hfirst Hfirst' HreadyD HreadyD' HreadyDef HreadyDef'.
+
+  move: v H0=> [[cur prev]] [re_sch] [ir_count] [[def_pending def_mask]] [[disk_pending disk_mask]] [timer_pending timer_mask].
+  move: v'=> [[cur' prev']] [re_sch'] [ir_count'] [[def_pending' def_mask']] [[disk_pending' disk_mask']] [timer_pending' timer_mask'].    
+  move/rel_eqpair=>[H0] /rel_eqpair[H1] /rel_eqpair[] H2 /rel_eqpair[]/rel_eqpair[H3 H4] /rel_eqpair[] H5 H6.
+  rewrite !pair_rewr in H0 H1 H2 H3 H4 H5 H6.  
+
+  apply/rel_eqpair2. con.
+  apply/rel_eqpair2. con.
+  rewrite /initiate_handler !pair_rewr. ssa. 
+
+  move/rel_eqpair2 : H0=>[]. rewrite !pair_rewr.
+  move/eqsum_split.
+  case.
+  move=>[]i0'[]i1'[]->[]->_/publicRel_eq ->. rewrite !pair_rewr //.
+  move=>[]i0'[]i1'[]->[]->/publicRel_eq ->/publicRel_eq ->. rewrite !pair_rewr //.
+  apply/rel_eqpair2. con.
+
+  move/publicRel_eq : H2=>->.
+  move/rel_eqpair2 : H0=>[]. rewrite !pair_rewr.
+  move/eqsum_split.
+  case.
+  move=>[]i0'[]i1'[]->[]->_/publicRel_eq ->. rewrite !pair_rewr //.
+  move/publicRel_eq : H1=>->//.
+  move=>[]i0'[]i1'[]->[]->/publicRel_eq ->/publicRel_eq ->. rewrite !pair_rewr //.
+  move/publicRel_eq : H1=>->//.  
+  apply/rel_eqpair2. con.
+
+  move/rel_eqpair2 : H0=>[]. rewrite !pair_rewr.
+  move/eqsum_split.
+  case.
+  move=>[]i0'[]i1'[]->[]->_/publicRel_eq ->. rewrite !pair_rewr //.
+  move/publicRel_eq : H1=>->//.
+  move=>[]i0'[]i1'[]->[]->/publicRel_eq ->/publicRel_eq ->. rewrite !pair_rewr //.
+
+  apply/rel_eqpair2. con.
+  apply/rel_eqpair2. con. eauto. ssa.
+  apply/rel_eqpair2. con.
+  apply/rel_eqpair2. con. eauto. ssa.
+  apply/rel_eqpair2. con.
+
+  move/rel_eqpair2 : H6. case. rewrite !pair_rewr. move=>/publicRel_eq->//. 
+  move/rel_eqpair2 : H0=>[]. rewrite !pair_rewr.
+  move/eqsum_split.
+  case.
+  move=>[]i0'[]i1'[]->[]->_/publicRel_eq ->//. 
+  move=>[]i0'[]i1'[]->[]-> /publicRel_eq ->/publicRel_eq ->. ssa.
+
+  move/publicRel_eq : H4=>->//.  
+
+  move=>[]HreadyD'[]HreadyDef' Hfirst'.
+  rewrite Hfirst Hfirst'. exfalso.
+
+  clear Hready HreadyD Hready' Hfirst Hfirst'.
+  
+  move: v H0 HreadyD' HreadyDef HreadyDef'=> [[cur prev]] [re_sch] [ir_count] [[def_pending def_mask]] [[disk_pending disk_mask]] [timer_pending timer_mask].
+  move: v'=> [[cur' prev']] [re_sch'] [ir_count'] [[def_pending' def_mask']] [[disk_pending' disk_mask']] [timer_pending' timer_mask'].    
+  move/rel_eqpair=>[_] /rel_eqpair[_] /rel_eqpair[] HH /rel_eqpair[]/rel_eqpair[_ H4] /rel_eqpair[] /rel_eqpair[] _ H5 /rel_eqpair[] _ H6.
+  rewrite !pair_rewr in HH H4 H5 H6.  
+  move: HH H4 H5 H6. move=>/publicRel_eq->/publicRel_eq->/publicRel_eq->/publicRel_eq->. 
+
+  rewrite /I_ready /get_I_pending /get_pending' /get_I_bits /get_I_bits' /get_ic /get_ic_count /get_bool_state /bool_coding /get_I_mask /get_mask' /get_I_bits /get_I_bits' /get_ic /get_ic_count /get_bool_state /update_bool_state !pair_rewr /timeslice_live /get_ir_count /get_ic_count /get_bool_state !pair_rewr.
+  rewrite /I_ready /get_I_pending /get_pending' /get_I_bits /get_I_bits' /get_ic /get_ic_count /get_bool_state /bool_coding /get_I_mask /get_mask' /get_I_bits /get_I_bits' /get_ic /get_ic_count /get_bool_state /update_bool_state !pair_rewr /timeslice_live /get_ir_count /get_ic_count /get_bool_state.  
+  move/negP. rewrite !negb_and !negbK.
+  move/orP. case. move/orP. case.
+  intro.
+  move/andP. case. move/orP. case.
+  move=>b.
+  rewrite negb_or negbK. move/andP.
+  case. move=>c d.
+  move/negP. rewrite negb_and negb_or.
+  move/orP. case. rewrite d. ssa. rewrite d. ssa.
+  rewrite negb_and negbK orbC /=in b0.
+  by rewrite b0 in c.
+  move=>->.  rewrite negb_or negbK.
+  move/andP. case.
+  move=>b c. move/negP.
+  rewrite negb_and negb_or.
+  move/orP. case. ssa.
+  rewrite negb_and b. ssa. ssa.
+  move/orP. case.
+  move=>a. move/andP. case.
+  move/orP. case. move=>b.
+  rewrite !negb_or !negbK. move/andP. case.
+  rewrite a. ssa.
+  move=>b. rewrite !negb_or !negbK.
+  move/andP. case. rewrite a. ssa.
+  move=>a. move/andP. case. move/orP. case.
+  move=>b. rewrite !negb_or negbK.
+  move/andP. case. move=>c.
+  move=>d. rewrite d in a. done.
+  move=>b. rewrite b in a. done.
+
+  move=>[]HreadyD[]HreadyDef Hfirst.
+  move=>[[]HreadyD'[]Hfirst'|].
+  rewrite Hfirst Hfirst'. exfalso.
+
+  clear Hready Hready' Hfirst Hfirst'.
+  
+  move: v H0 HreadyD' HreadyD HreadyDef => [[cur prev]] [re_sch] [ir_count] [[def_pending def_mask]] [[disk_pending disk_mask]] [timer_pending timer_mask].
+  move: v'=> [[cur' prev']] [re_sch'] [ir_count'] [[def_pending' def_mask']] [[disk_pending' disk_mask']] [timer_pending' timer_mask'].    
+  move/rel_eqpair=>[_] /rel_eqpair[_] /rel_eqpair[] HH /rel_eqpair[]/rel_eqpair[_ H4] /rel_eqpair[] /rel_eqpair[] _ H5 /rel_eqpair[] _ H6.
+  rewrite !pair_rewr in HH H4 H5 H6.  
+  move: HH H4 H5 H6. move=>/publicRel_eq->/publicRel_eq->/publicRel_eq->/publicRel_eq->. 
+
+  rewrite /I_ready /get_I_pending /get_pending' /get_I_bits /get_I_bits' /get_ic /get_ic_count /get_bool_state /bool_coding /get_I_mask /get_mask' /get_I_bits /get_I_bits' /get_ic /get_ic_count /get_bool_state /update_bool_state !pair_rewr /timeslice_live /get_ir_count /get_ic_count /get_bool_state !pair_rewr.
+  rewrite /I_ready /get_I_pending /get_pending' /get_I_bits /get_I_bits' /get_ic /get_ic_count /get_bool_state /bool_coding /get_I_mask /get_mask' /get_I_bits /get_I_bits' /get_ic /get_ic_count /get_bool_state /update_bool_state !pair_rewr /timeslice_live /get_ir_count /get_ic_count /get_bool_state.  
+  move/andP. case. intro.
+  rewrite negb_or negbK. move/andP. case.
+  intro. intro.
+  move/negP. rewrite negb_and negb_or.
+  move/orP. case. move/andP. case.
+  move=> c _.
+  move/negP. rewrite negb_and negb_or.
+  move/orP. case. move/andP. case.
+  intro. rewrite b. done. rewrite negb_and negbK.
+  move/orP. case. intro. rewrite a1 in a0. done.
+  rewrite b. done. rewrite negb_and negbK.
+  move/orP. case. intro. rewrite a1 in a0. done.
+  rewrite b. done.
+
+  move=>[[]HreadyD'[]HreadyDef' Hfirst'|].
+  rewrite Hfirst Hfirst'. exfalso.
+
+  clear Hready Hready' Hfirst Hfirst'.
+  
+  move: v H0 HreadyD' HreadyD HreadyDef HreadyDef' => [[cur prev]] [re_sch] [ir_count] [[def_pending def_mask]] [[disk_pending disk_mask]] [timer_pending timer_mask].
+  move: v'=> [[cur' prev']] [re_sch'] [ir_count'] [[def_pending' def_mask']] [[disk_pending' disk_mask']] [timer_pending' timer_mask'].    
+  move/rel_eqpair=>[_] /rel_eqpair[_] /rel_eqpair[] HH /rel_eqpair[]/rel_eqpair[_ H4] /rel_eqpair[] /rel_eqpair[] _ H5 /rel_eqpair[] _ H6.
+  rewrite !pair_rewr in HH H4 H5 H6.  
+  move: HH H4 H5 H6. move=>/publicRel_eq->/publicRel_eq->/publicRel_eq->/publicRel_eq->. 
+
+  rewrite /I_ready /get_I_pending /get_pending' /get_I_bits /get_I_bits' /get_ic /get_ic_count /get_bool_state /bool_coding /get_I_mask /get_mask' /get_I_bits /get_I_bits' /get_ic /get_ic_count /get_bool_state /update_bool_state !pair_rewr /timeslice_live /get_ir_count /get_ic_count /get_bool_state !pair_rewr.
+  rewrite /I_ready /get_I_pending /get_pending' /get_I_bits /get_I_bits' /get_ic /get_ic_count /get_bool_state /bool_coding /get_I_mask /get_mask' /get_I_bits /get_I_bits' /get_ic /get_ic_count /get_bool_state /update_bool_state !pair_rewr /timeslice_live /get_ir_count /get_ic_count /get_bool_state.
+
+  move/negP. rewrite !negb_and !negb_or.
+  move/orP. case. intro.
+
+  move/negP. rewrite ?negb_and ?negb_or.
+  move/orP. case. intro.
+
+  move/negP. rewrite ?negb_and ?negb_or.
+  move/orP. case. move/andP. case. intro. intro.
+
+  move/andP. case. move/orP. case. intro.
+  move/andP. case. intro. rewrite b. done.
+  intro. rewrite b0 in b. done.
+  rewrite !negbK.
+  move/orP. case. intro.
+  move/andP. case.
+  move/orP. case. intro.
+  move/andP. case. intro. rewrite a1 in a3. done.
+  intro.
+  rewrite b a1. done.
+  intro. move/andP. case.
+  move/orP. case. intro.
+  move/andP. case. intro. intro. rewrite b0 in b. done.
+  intro. rewrite b0 in b. done.
+  rewrite !negbK. move/orP. case. intro.
+  move/negP. rewrite !negb_and !negb_or.
+  move/orP. case. move/andP. case. intro.
+  intro. move/andP. case. move/orP. case.
+  intro. move/andP. case. intro.
+  intro. rewrite b0 in b. done.
+  intro. rewrite b0 in b. done.
+  rewrite negbK. rewrite a0. simpl. 
+  move=>_. move/andP. ssa. intro.
+  move/negP. rewrite negb_and negb_or.
+  move/orP. case. move/andP. case. intro. rewrite b.
+  move=>_. move/andP. case. move/orP. case.
+  intro. move/andP. case. intro. intro. rewrite b0 in b. done.
+  intro. rewrite b0 in b. done.
+  rewrite negb_and negbK. move/orP. case. intro. move/andP.
+  case. move/orP. case. intro. move/andP.  rewrite a0. ssa.
+  intro. rewrite b0 in b. done.
+  move=>_. move/andP. case. move/orP. case. intro.
+  move/andP. case. intro. intro. rewrite b0 in b. done.
+  intro. rewrite b0 in b. done.
+  rewrite !negb_and !negbK. move/orP. case.
+  intro. 
+  move/negP.
+  rewrite !negb_and negbK.
+  move/orP. case.
+  move/orP. case. intro.
+  move/negP. rewrite negb_and negb_or.
+  move/orP. case.
+  move/andP. case. intro. intro.
+  move/andP. case.
+  move/orP. case.
+  intro. move/andP. case. intro. intro. rewrite b0 in b. done.
+  intro. rewrite b0 in b. done.
+  rewrite !negb_and negbK. move/orP. case.
+  intro.
+  move/andP. case. move/orP. case.
+  intro. move/andP. case. rewrite a1. done.
+  move=>->. rewrite a1. done.
+  intro. move/andP. case.
+  move/orP. case. intro. move/andP. case.
+  rewrite a. done.
+  intro. rewrite b0 in b. done.
+  done. move/orP. case. intro.
+  move/negP. rewrite negb_and negb_or.
+  rewrite negb_and.
+  move/orP. case. move/andP. case.
+  intro. intro. move/andP. case.
+  move/orP. case. intro. rewrite a. done.
+  intro. rewrite b0 in b. done.
+  rewrite negbK. move/orP. case. intro.
+  move/andP. case. move/orP. case.
+  intro. move/andP. case. intro. rewrite a in a3. done.
+  move=>->. rewrite a. done.
+  intro. move/andP. case.
+  move/orP. case. intro.
+  move/andP. case. intro. intro. rewrite b0 in b. done.
+  intro. rewrite b0 in b. done.
+  intro.
+  move/negP. rewrite negb_and negb_or.
+  move/orP. case. move/andP. case.
+  intro. intro.
+  move/andP. case. move/orP. case.
+  intro. move/andP. case. intro.
+  intro. rewrite b1 in b0. done.
+  intro. rewrite b1 in b0. done.
+  rewrite !negb_and negbK. move/orP. case.
+  intro. move/andP. case.
+  move/orP. case. intro. move/andP. case.
+  rewrite a0. done.
+  intro. rewrite b0 in b. done.
+  intro. move/andP. case. move/orP. case.
+  intro. move/andP. case. intro.
+  intro. rewrite b1 in b. done.
+  intro. rewrite b1 in b. done.
+  intro. 
+  move/negP. rewrite negb_and negb_or.
+  move/orP. case. move/andP. case. intro.
+  intro.
+  move/negP. rewrite !negb_and. move/orP. 
+  rewrite negb_or.
+  case. move/andP. case. intro.
+  intro. move/andP. case. move/orP. case.
+  intro. move/andP. case. intro. intro. rewrite b2 in b1. done.
+  intro. rewrite b2 in b1. done.
+  rewrite negbK. move/orP. case. intro.
+  move/andP. case. move/orP. case. intro.
+  move/andP. case. intro. intro. rewrite b1 in b. done.
+  intro. rewrite b1 in b. move/andP. rewrite a0. ssa.
+  intro.
+  move/andP. case. move/orP. case.
+  move=>b2. move/andP. case. intro. intro.
+  rewrite b3 in b1. done.
+  intro. rewrite b2 in b1. done.
+  rewrite negb_and !negbK. move/orP. case.
+  intro.
+  move/negP. case.
+  rewrite !negb_and negb_or.
+  move/orP. case.
+  move/andP. case. intro. intro. move/andP. case.
+  move/orP. case. intro. rewrite a. ssa.
+  intro. rewrite b1 in b0. done.
+  rewrite negbK. rewrite a. ssa.
+  intro.
+  move/negP. rewrite negb_and negb_or.
+  move/orP. case. move/andP. case.
+  intro. intro. move/andP. case.
+  move/orP. case. intro.
+  move/andP. case. intro. intro. rewrite b2 in b1. done.
+  intro. rewrite b2 in b1. done.
+  rewrite negb_and negbK. move/orP. case.
+  intro. move/andP. case. move/orP.
+  case. intro. move/andP. case. rewrite a. done.
+  intro. rewrite b1 in b. done.
+  intro. move/andP. case.
+  move/orP. case. intro. move/andP. case.
+  intro. intro. rewrite b2 in b. done.
+  intro. rewrite b2 in b. done.
+
+  move=>[]HreadyD'[]HreadyDef' Hfirst'.
+  rewrite Hfirst Hfirst'.
+
+  clear Hready Hready' HreadyD HreadyDef Hfirst HreadyD' HreadyDef' Hfirst'.
+
+  have: is_handler_pid (bool_coding v) = is_handler_pid (bool_coding v').
+  move: v H0=> [[cur prev]] [re_sch] [ir_count] [[def_pending def_mask]] [[disk_pending disk_mask]] [timer_pending timer_mask].
+  move: v'=> [[cur' prev']] [re_sch'] [ir_count'] [[def_pending' def_mask']] [[disk_pending' disk_mask']] [timer_pending' timer_mask'].  
+
+  move/rel_eqpair=>[H0] /rel_eqpair[H1] /rel_eqpair[] H2 /rel_eqpair[]/rel_eqpair[H3 H4] /rel_eqpair[] H5 H6.
+  rewrite !pair_rewr in H0 H1 H2 H3 H4 H5 H6.
+
+  move: H0.
+  case/rel_eqpair. rewrite !pair_rewr.
+  move=>+ /publicRel_eq ->.
+
+  move/eqsum_split.
+  case.
+  move=>[]i0'[]i1'[]->[]->_. ssa.
+  move=>[]i0'[]i1'[]->[]->/publicRel_eq ->. ssa.
+  move=>->.
+  destruct (is_handler_pid _).
+  have: get_re_sch (bool_coding v) = get_re_sch (bool_coding v').
+  move: v H0=> [[cur prev]] [re_sch] [ir_count] [[def_pending def_mask]] [[disk_pending disk_mask]] [timer_pending timer_mask].
+  move: v'=> [[cur' prev']] [re_sch'] [ir_count'] [[def_pending' def_mask']] [[disk_pending' disk_mask']] [timer_pending' timer_mask'].
+
+  move/rel_eqpair=>[H0] /rel_eqpair[H1] /rel_eqpair[] H2 /rel_eqpair[]/rel_eqpair[H3 H4] /rel_eqpair[] H5 H6.
+  rewrite !pair_rewr in H0 H1 H2 H3 H4 H5 H6.
+  move/rel_eqpair : H0. case. rewrite !pair_rewr.
+
+  move=>+ /publicRel_eq ->.
+  move/publicRel_eq : H1=>->.
+
+  move/eqsum_split.
+  case.
+  move=>[]i0'[]i1'[]->[]->_. ssa.
+  move=>[]i0'[]i1'[]->[]->/publicRel_eq ->. ssa.
+
+  move=>->.
+  destruct (get_re_sch (bool_coding v')).
+
+  move: v H0=> [[cur prev]] [re_sch] [ir_count] [[def_pending def_mask]] [[disk_pending disk_mask]] [timer_pending timer_mask].
+  move: v'=> [[cur' prev']] [re_sch'] [ir_count'] [[def_pending' def_mask']] [[disk_pending' disk_mask']] [timer_pending' timer_mask'].    
+  move/rel_eqpair=>[H0] /rel_eqpair[H1] /rel_eqpair[] H2 /rel_eqpair[]/rel_eqpair[H3 H4] /rel_eqpair[] H5 H6.
+  rewrite !pair_rewr in H0 H1 H2 H3 H4 H5 H6.  
+
+  apply/rel_eqpair2. con.
+  apply/rel_eqpair2. con. rewrite !pair_rewr. done. done.
+  apply/rel_eqpair2. con. done.
+  apply/rel_eqpair2. con. done.
+  apply/rel_eqpair2. con.
+  apply/rel_eqpair2. con.  eauto. rewrite !pair_rewr.
+
+  move/publicRel_eq : H4=>->.
+  move/rel_eqpair2 : H5.
+  case. rewrite !pair_rewr. move=>_ /publicRel_eq ->//.
+  move/publicRel_eq :H2=>->. done.
+  apply/rel_eqpair2. con.
+  apply/rel_eqpair2. con. done. 
+  move/publicRel_eq : H2=>->. rewrite !pair_rewr.
+  move/rel_eqpair2 : H5. case. rewrite !pair_rewr. move=>_ /publicRel_eq ->. ssa.
+  apply/rel_eqpair2. con. rewrite !pair_rewr.
+  move/rel_eqpair2 : H6. case. rewrite !pair_rewr.
+  move/publicRel_eq ->. done.
+  rewrite !pair_rewr.
+  move/rel_eqpair2 : H6. case. rewrite !pair_rewr.
+  move=>/publicRel_eq -> /publicRel_eq ->//.
+  move/publicRel_eq : H2=>->//.
+
+
+  move: v H0=> [[cur prev]] [re_sch] [ir_count] [[def_pending def_mask]] [[disk_pending disk_mask]] [timer_pending timer_mask].
+  move: v'=> [[cur' prev']] [re_sch'] [ir_count'] [[def_pending' def_mask']] [[disk_pending' disk_mask']] [timer_pending' timer_mask'].    
+  move/rel_eqpair=>[H0] /rel_eqpair[H1] /rel_eqpair[] H2 /rel_eqpair[]/rel_eqpair[H3 H4] /rel_eqpair[] H5 H6.
+  rewrite !pair_rewr in H0 H1 H2 H3 H4 H5 H6.    
+
+  move/rel_eqpair : H0. case. rewrite !pair_rewr.
+  move=>_ /publicRel_eq ->.
+  move/publicRel_eq : H1=>->.
+  move/publicRel_eq : H2=>->.
+  move/publicRel_eq : H4=>->.  ssa.
+  rewrite /odflt /oapp /get_prev_pid /get_prev_pid_wrap /get_prev_pid /get_pids !pair_rewr.
+  destruct prev'. done.
+  destruct scheduler_pid. auto. done.
+  subst. cbv. case_if. done.
+  destruct ir_count'. done. done.
+  subst. ssa. subst. done. subst. done.
+
+  
+  move: v H0=> [[cur prev]] [re_sch] [ir_count] [[def_pending def_mask]] [[disk_pending disk_mask]] [timer_pending timer_mask].
+  move: v'=> [[cur' prev']] [re_sch'] [ir_count'] [[def_pending' def_mask']] [[disk_pending' disk_mask']] [timer_pending' timer_mask'].    
+  move/rel_eqpair=>[H0] /rel_eqpair[H1] /rel_eqpair[] H2 /rel_eqpair[]/rel_eqpair[H3 H4] /rel_eqpair[] H5 H6.
+  rewrite !pair_rewr in H0 H1 H2 H3 H4 H5 H6.    
+
+  ssa. subst. done.
+  subst. cbv. case_if. done.
+  destruct ir_count'. done. done. subst. done. subst. done.
+  subst. done.
+
+
+  
+  apply f_EP_comp.
+
+  rewrite /step0.
+  mrw. intro.
+  intro. destruct i.
+  intro. have: dis in_rel l i. ssa. clear H=>H.
+  intros.
+  rewrite /step_left.
+  simpl in H. rewrite /ir_dis in H. destruct H. subst.
+
+  move: v => [[cur prev]] [re_sch] [ir_count] [[def_pending def_mask]] [[disk_pending disk_mask]] [timer_pending timer_mask].
+  apply/rel_eqpair2. con. rewrite !pair_rewr. ssa. de cur.
+  apply/rel_eqpair2. con. rewrite !pair_rewr. ssa.
+  apply/rel_eqpair2. con. rewrite !pair_rewr. ssa.
+  apply/rel_eqpair2. con. rewrite !pair_rewr. ssa.
+  apply/rel_eqpair2. con. rewrite !pair_rewr. ssa.
+  apply/rel_eqpair2. con. rewrite !pair_rewr. ssa. ssa.
+  ssa.
+
+  apply f_EP_comp.
+  rewrite /step1.
+  mrw. intros.
+  destruct i. have: (step_right check_scheduler (inl i) v) = v. done. move=>->//.
+  ssa.
+
+  apply f_EP_comp.
+  mrw. intros.
+  destruct i. have: (step_right good_preroutine (inl i) v) = v. done. move=>->//.
+  ssa.
+
+  mrw. intros.
+  destruct i.
+  have:  (step_right (fun=> initiate_next bool_coding) (inl i) v) = v. done.
+  move=>->. auto.
+  ssa.
+
+  (*map*)
+  eapply map_NI.
+  instantiate (1:= eqmaybe_false (eqpair (eqsum (semiprivateRel Bool) (publicRel _)) (eqmaybe_false (semiprivateRel _)))).
+  mrw. intros.
+  destruct i. destruct i'.
+  rewrite !pair_rewr.
+  apply rel_eqpair_R2' in H.
+  destruct H. destruct H.
+  remember H0. clear Heqr.
+  move/eqsum_split : H0. case.
+  move=>[]x0[]x1[]->[]->. auto.
+  move=>[]x0[]x1[]->[]->Hout.
+  apply rel_eqmaybe_false2.
+  apply rel_eqpair2. con. rewrite !pair_rewr.
+
+  move:H.
+  move/rel_eqpair=>[] /rel_eqpair[]//.
+  rewrite !pair_rewr.
+
+  move:Hout.
+  move/rel_eqpair=>[] _ /rel_eqpair[] _ /rel_eqpair[] _ /rel_eqpair[] _ /rel_eqpair[] Hout _.
+  move:Hout.
+  case: x0=>a[]b[]c[]d[] e f.
+  case: x1=>a'[]b'[] c'[] d'[] e' f'.
+  rewrite !pair_rewr.
+  move/rel_eqmaybe_top. case.
+  move=>[]x'[]y'[] ->[]->.
+  rewrite /dI_out. intro. move: b0. simpl. case.
+  case. intros. subst. auto. intros. auto.
+
+  case.
+  move=>[]x'[]y'[] ->[]->. intros. simpl. de e. case.
+  move=>[]y'[] ->[]->. case. intros. subst. ssa.
+  case. move=>->->. auto.
+  case:H.
+  destruct i0;last ssa.
+  destruct i2;last ssa.
+  auto.
+
+  mrw. intros. destruct i. apply dis_eqpair_R in H. destruct i0;last ssa.
+  rewrite !pair_rewr. done.
+
+  mrw. intros. 
+  apply rel_eqsum_L2. eapply H.  
+  
+  eapply maybe_NI.
+  eapply par_NI.
+  eapply map_NI.
+  instantiate (1:= eqpair_LR falseRel (_)).
+  mrw. intros. apply rel_eqpair in H. destruct H.
+  apply rel_eqpair_LR2. con. 2:eauto.
+  clear H0.
+  case/eqsum_split:H.
+  move=>[]x[]y[]->[]->. intros.
+  simpl in b. destruct b. destruct H. subst. eauto.
+  subst. simpl. case_if. case_if. done. done.
+  case_if. done. done.
+  move=>[]x[]y[]->[]->/publicRel_eq->/=. done.
+  mrw. intros. ssa.
+  instantiate (1:= eqmaybe_swi (publicRel _) falseRel).
+  mrw. intros. apply rel_eqmaybe_swi2 in H.
+  destruct H. destruct H. destruct H. destruct H. destruct H0.
+  subst. apply rel_eqmaybe. eauto.
+  destruct H. destruct H. subst. auto.
+  destruct H. destruct i. ssa. destruct i'. ssa. auto.
+
+  apply swi_NI.
+  intros. left. intro. intros.
+  simpl in H. subst. ssa. intro. ssa.
+  
+  eapply maybe_NI. eapply map_NI. eauto. eauto.
+  mrw. intros. apply rel_eqpair_LR2. con. auto. eauto.
+  apply out_NI.
+  
+
+  apply par_NI.
+  (*map*)
+
+  eapply map_NI.
+  instantiate (1:= eqpair_LR falseRel _).
+  mrw. intros. apply rel_eqpair in H. destruct H.
+  apply rel_eqpair_LR2. con. 
+  clear H0.
+  case/eqsum_split:H.
+  move=>[]x[]y[]->[]->. intros.
+  simpl in b. destruct b. destruct H. subst. eauto.
+  subst. simpl. case_if. case_if. done. done.
+  case_if. done. done.
+  move=>[]x[]y[]->[]->/publicRel_eq->/=. done. eauto.
+  mrw. intros. ssa.
+  instantiate (1:= eqmaybe_swi (semiprivateRel _) falseRel).
+  mrw. intros. apply rel_eqmaybe_swi2 in H.
+  destruct H. destruct H. destruct H. destruct H. destruct H0.
+  subst. apply rel_eqmaybe. eauto.
+  destruct H. destruct H. subst. auto.
+  destruct H. destruct i. ssa. destruct i'. ssa. ssa. intro. apply H0. intro. ssa. subst.
+  intro. ssa. de i'. intro. apply H. intro. ssa. intro. apply H. intro. intros. subst.
+  ssa. 
+
+  apply swi_NI.
+  intros. left. intro. intros.
+  simpl in H. subst. ssa. intro. ssa.
+  
+  eapply maybe_NI. eapply map_NI. eauto. eauto.
+  mrw. intros. apply rel_eqpair_LR2. con. auto. eauto.
+
+  eapply map_NI.
+  mrw. intros. apply rel_eqsum_L. eauto.
+  mrw. intros. apply dis_eqsum_L. done.
+  mrw. intros. move: H.
+  instantiate (1:= eqsum_L _ _). intros.
+  destruct i. destruct i'. apply rel_refl. ssa.
+  destruct i'. ssa.
+  apply rel_eqsum_R2' in H.
+  destruct i. destruct i0.
+  2: apply loop_NI.
+  destruct i1. destruct i2.
+  move:H. instantiate (1:=  (eqpair (semiprivateRel Bool) _)).
+  move/rel_eqpair. case. rewrite !pair_rewr.
+  intros. clear b. ssa. destruct a. ssa. subst. case_if. subst. ssa. subst. ssa.
+  ssa.
+
+  
+  eapply map_NI.
+  apply f_NI_id.
+  apply f_PU_id.
+
+  mrw. intros. apply rel_eqsum_L2. eauto.
+
+  apply sta_NI.
+  mrw. intros. eauto.
+  mrw. intros.
+  destruct i. destruct i'. apply rel_eqsum_L' in H.
+  ssa. de H. de H0. subst. left. ssa.
+  ssa. destruct i'. ssa. apply rel_refl.
+  mrw. intros. destruct i. apply dis_eqsum_L2 in H. ssa. ssa.
+  apply out_NI.
+  
+  apply par_NI.
+  (*map*)
+
+  eapply map_NI.
+  instantiate (1:= eqpair_LR falseRel _).
+  mrw. intros. apply rel_eqpair in H. destruct H.
+  apply rel_eqpair_LR2. con. 
+  clear H0.
+  case/eqsum_split:H.
+  move=>[]x[]y[]->[]->. intros.
+  simpl in b. destruct b. destruct H. subst. eauto.
+  subst. simpl. case_if. case_if. done. done.
+  case_if. done. done.
+  move=>[]x[]y[]->[]->/publicRel_eq->/=. done. eauto.
+  mrw. intros. ssa.
+  instantiate (1:= eqmaybe_swi (publicRel _) falseRel).
+  mrw. intros. apply rel_eqmaybe_swi2 in H.
+  destruct H. destruct H. destruct H. destruct H. destruct H0.
+  subst. apply rel_eqmaybe. eauto.
+  destruct H. destruct H. subst. auto.
+  destruct H. destruct i. ssa. destruct i'. ssa. ssa.
+  
+  apply swi_NI.
+  intros. left. intro. intros.
+  simpl in H. subst. ssa. intro. ssa.
+  
+  eapply maybe_NI. eapply map_NI. eauto. eauto.
+  mrw. intros. apply rel_eqpair_LR2. con. auto. eauto.
+
+  eapply map_NI. eauto. eauto.
+  instantiate (1:=eqpair _ _).
+  mrw. move=> l i i' /rel_eqpair[] + _.
+  instantiate (1:= publicRel _). move=>/publicRel_eq ->. ssa.
+  eapply sta_NI.
+  mrw. intros. move: H0.
+  move/publicRel_eq=>->//.
+  mrw. intros. eauto.
+  mrw. intros. auto.
+  apply out_NI.
+
+  apply par_NI.
+  (*map*)
+
+  eapply map_NI.
+  instantiate (1:= eqpair_LR (semiprivateRel _) _).
+  mrw. intros. apply rel_eqpair in H. destruct H.
+  apply rel_eqpair_LR2. con. 
+  clear H0.
+  case/eqsum_split:H.
+  move=>[]x[]y[]->[]->. intros.
+  simpl in b. destruct b. destruct H. subst. eauto. eauto.
+  move=>[]x[]y[]->[]->/publicRel_eq->/=.
+  destruct (eqVneq l \bot). auto. left. ssa. intro. apply/negP. apply i0. apply/eqP. done.
+  instantiate (1:= eqmaybe_false (semiprivateRel _)). auto.
+  mrw. intros. ssa.
+  instantiate (1:= eqmaybe_swi (semiprivateRel _) (semiprivateRel _)).
+  mrw. intros. apply rel_eqmaybe_swi2 in H.
+  destruct H. destruct H. destruct H. destruct H. destruct H0.
+  subst. apply rel_eqmaybe. eauto.
+  destruct H. destruct H. subst. auto.
+  destruct H. destruct i. ssa. destruct i'. ssa. ssa. de i'.
+  
+  apply swi_NI.
+  intros.
+  destruct (eqVneq l \bot). subst. right.
+  intro. intros.
+  elim: H. intros. con.
+  intros. econ. done.
+  intros. econ. 2:done. ssa.
+  left. intro. intros.
+  move/semiprivate_not_bot' : H=>->//. ssa.
+  intro. subst. rewrite eqxx in i. done.
+  intro. subst. rewrite eqxx in i. done.
+
+  apply maybe_NI.
+  eapply map_NI. eauto. eauto.
+
+  mrw. intros. apply rel_eqpair_LR2. con. auto. eauto.
+
+  eapply map_NI. eauto. eauto.
+  mrw. intros.
+  move:H. instantiate (1:=eqpair (semiprivateRel _) (publicRel _)).
+  move/rel_eqpair. case=>HH _.
+  simpl in HH. destruct HH. destruct H. rewrite H0.
+  case_if. auto. auto. subst. auto.
+  
+  eapply sta_NI.
+  mrw. intros. simpl in H0. destruct H0. ssa. subst. auto.
+  mrw. intros. auto.
+  mrw. intros. auto.
+  apply out_NI.
+
+
+  apply par_NI.
+  (*map*)
+
+  eapply map_NI.
+  instantiate (1:= eqpair_LR (semiprivateRel _) _).
+  mrw. intros. apply rel_eqpair in H. destruct H.
+  apply rel_eqpair_LR2. con. 
+  clear H0.
+  case/eqsum_split:H.
+  move=>[]x[]y[]->[]->. intros.
+  simpl in b. destruct b. destruct H. subst. eauto. eauto.
+  move=>[]x[]y[]->[]->/publicRel_eq->/=.
+  destruct (eqVneq l \bot). auto. left. ssa. intro. apply/negP. apply i0. apply/eqP. done.
+  instantiate (1:= eqmaybe_false (semiprivateRel _)). auto.
+  mrw. intros. ssa.
+  instantiate (1:= eqmaybe_swi (semiprivateRel _) (semiprivateRel _)).
+  mrw. intros. apply rel_eqmaybe_swi2 in H.
+  destruct H. destruct H. destruct H. destruct H. destruct H0.
+  subst. apply rel_eqmaybe. eauto.
+  destruct H. destruct H. subst. auto.
+  destruct H. destruct i. ssa. destruct i'. ssa. ssa. de i'.
+  
+  apply swi_NI.
+  intros.
+  destruct (eqVneq l \bot). subst. right.
+  intro. intros.
+  elim: H. intros. con.
+  intros. econ. done.
+  intros. econ. 2:done. ssa.
+  left. intro. intros.
+  move/semiprivate_not_bot' : H=>->//. ssa.
+  intro. subst. rewrite eqxx in i. done.
+  intro. subst. rewrite eqxx in i. done.
+
+  apply maybe_NI.
+  eapply map_NI. eauto. eauto.
+
+  mrw. intros. apply rel_eqpair_LR2. con. auto. eauto.
+
+  eapply map_NI. eauto. eauto.
+  mrw. intros.
+  move:H. instantiate (1:=eqpair (semiprivateRel _) (publicRel _)).
+  move/rel_eqpair. case=>HH _.
+  simpl in HH. destruct HH. destruct H. rewrite H0.
+  case_if. auto. auto. subst. auto.
+  
+  eapply sta_NI.
+  mrw. intros. simpl in H0. destruct H0. ssa. subst. auto.
+  mrw. intros. auto.
+  mrw. intros. auto.
+  apply out_NI.
+
+  eapply map_NI.
+  instantiate (1:= eqpair_LR falseRel _).
+  mrw. intros. apply rel_eqpair in H. destruct H.
+  apply rel_eqpair_LR2. con. 
+  clear H0.
+  case/eqsum_split:H.
+  move=>[]x[]y[]->[]->. intros.
+  simpl in b. destruct b. destruct H. subst. eauto.
+  subst. simpl. case_if. case_if. done. done.
+  case_if. done. done.
+  move=>[]x[]y[]->[]->/publicRel_eq->/=. done. eauto.
+  mrw. intros. ssa.
+  instantiate (1:= eqmaybe_swi (publicRel _) falseRel).
+  mrw. intros. apply rel_eqmaybe_swi2 in H.
+  destruct H. destruct H. destruct H. destruct H. destruct H0.
+  subst. apply rel_eqmaybe. eauto.
+  destruct H. destruct H. subst. auto.
+  destruct H. destruct i. ssa. destruct i'. ssa. ssa.
+  
+  apply swi_NI.
+  intros. left. intro. intros.
+  simpl in H. subst. ssa. intro. ssa.
+  
+  eapply maybe_NI. eapply map_NI. eauto. eauto.
+  mrw. intros. apply rel_eqpair_LR2. con. auto. eauto.
+
+  eapply map_NI. eauto. eauto.
+  instantiate (1:=eqpair _ _).
+  mrw. move=> l i i' /rel_eqpair[] + _.
+  instantiate (1:= publicRel _). move=>/publicRel_eq ->. ssa.
+  eapply sta_NI.
+  mrw. intros. move: H0.
+  move/publicRel_eq=>->//.
+  mrw. intros. eauto.
+  mrw. intros. auto.
+  apply out_NI.
+
+  Unshelve. all: apply publicRel.
+Qed.  
+
+
+Lemma wrapped_model_good_NI : NI in_rel final_out_rel wrapped_model_good.
+Proof.
+  eapply map_NI. eauto. eauto.
+  2: apply model_good_NI.
+  mrw. intros.
+  move: H=> /rel_eqpair[] + /rel_eqpair[] + /rel_eqpair[] + /rel_eqpair[] + /rel_eqpair[] + +.
+  move: i=>[a[] b[] c[] d[] e f].
+  move: i'=>[a'[] b'[] c'[] d'[] e' f']. 
+  rewrite !pair_rewr.
+  rewrite /parse_output.
+  move/rel_eqmaybe2. case.
+  move=>[]x'[]y'[]->[]->/publicRel_eq->//.
+  move=>[]->->.
+  move/rel_eqmaybe2. case.
+  move=>[]x'[]y'[]->[]-> H _ _ _ _.
+  apply rel_eqmaybe. ssa.
+  move=>[]->[]->. auto.
+Qed.  
